Daily commit

theories/Translation.v
@@ -256,6 +256,15 @@ Section Translation.
       all: rasimpl.
       + 
   Admitted.
+
+  (* required for tl_subst_ignore *)
+  (* might require `swf Γ` *)
+  Lemma conv_stype_sort Γ A B s i :
+    A ≡ B →
+    Γ ⊢ A : Sort s i →
+    Γ ⊢ B : Sort s i.
+  Proof.
+  Admitted.
     
   Lemma tl_subst_ignore Γ t A i σ τ :
     swf Γ →
@@ -353,143 +362,73 @@ Section Translation.
     - apply IHh1_1 with (i := i).
       1, 3: assumption.
       clear h1_2. clear IHh1_2.
-      admit.
-  Admitted.
+      eapply conv_stype_sort.
+      2: eassumption.
+      now apply conv_sym.
+  Qed.
     
-  Lemma tl_subst_Typ Γ A B u v j :
+  Lemma tl_subst_Typ Γ A B u v i j :
     swf Γ →
+    Γ ⊢ A : Typ i → 
     Γ,,s (S_Typ, A) ⊢ B : PTyp j →
     [sc (Γ,,s (S_Typ, A)) | B] <[ u.. ] =
     [sc (Γ,,s (S_Typ, A)) | B] <[ v.. ].
   Proof.
-    intros hΓ h.
-    remember (Γ,,s (S_Typ, A)) as Δ eqn: eΔ.
-    remember (PTyp j) as C eqn: eC.
-    induction h using styping_ind in Γ, A, u, v, j, hΓ, eC, eΔ |- *.
-    all: subst.
-    - simpl.
-      unfold isPTyp.
-      change (S_Typ :: sc Γ) with (sc (Γ,,s (S_Typ, A))).
-      unfold sc. rewrite nth_error_map, H.
-      simpl. destruct s.
-      1: reflexivity.
-      destruct x.
-      + simpl in H. injection H.
-        discriminate.
-      + reflexivity.
-    - simpl. destruct s; reflexivity.
-    - injection eC; intros <- ->; clear eC.
-      simpl in *.
-      destruct s; simpl.
-      + f_equal.
-        admit.
-      + (*rewrite IHh1 with (v := v).*)
-
-    (*
-    inversion h.
-    - simpl.
-      unfold isPTyp.
-      change (S_Typ :: sc Γ) with (sc (Γ,,s (S_Typ, A))).
-      unfold sc. rewrite nth_error_map, H1.
-      simpl. destruct s.
-      1: reflexivity.
-      destruct x.
-      + simpl in H1. injection H1.
-        discriminate.
-      + reflexivity.
+    intros hΓ hA hB.
+    apply tl_subst_ignore with (A := PTyp j) (i := S j).
+    1, 3: econstructor; eassumption.
+    1: assumption.
+    intros x hx.
+    destruct x.
+    - apply scoping_st in hx.
+      simpl in hx; discriminate.
     - reflexivity.
-    - destruct s; simpl.
-  Admitted.
+  Qed.
 
-    remember (Γ,,s (S_Typ, A)) as Δ eqn: eΔ.
-    remember (PTyp j) as C eqn: eC.
-    induction h using styping_ind in u, v, hΓ, eC, eΔ |- *.
-    all: subst.
-    - simpl.
-      unfold isPTyp.
-      change (S_Typ :: sc Γ) with (sc (Γ,,s (S_Typ, A))).
-      unfold sc. rewrite nth_error_map, H.
-      simpl. destruct s.
-      1: reflexivity.
-      destruct x.
-      + simpl in H. injection H.
-        discriminate.
-      + reflexivity.
-    - simpl. destruct s; reflexivity.
-    - injection eC; intros <- ->; clear eC.
-      simpl in *.
-      destruct s; simpl.
-      + f_equal.
-        admit.
-      + rewrite IHh1 with (v := v).
-      
-  Lemma test Γ A B u i j :
-    swf Γ →
-    Γ ⊢ u : A →
-    Γ ⊢ A : Typ i →
-    Γ,,s (S_Typ, A) ⊢ B : PTyp j →
-    [sc (Γ,,s (S_Typ, A)) | B] <[ [sc Γ | u].. ] =
-    [sc (Γ,,s (S_Typ, A)) | B] <[ tt.. ].
-  Proof.
-    intros hΓ h1 h2 h3.
-    assert (scoping (sc Γ) u S_Typ) as h'.
-    {
-      change S_Typ with (stc Γ (Typ i)).
-      rewrite <-(styping_stc _ A).
-      2, 3: assumption.
-      now apply styping_scoping_stc.
-    }
-    destruct (tl_unit_tt _ _ h').
-    1: now rewrite H.
-    rewrite H; clear H.
-    remember (Γ,,s (S_Typ, A)) as Δ eqn: eΔ.
-    remember (PTyp j) as C eqn: eC.
-    induction h3 using styping_ind in
-      u, i, hΓ, h1, h2, h', eC, eΔ |- *.
-    all: subst.
-    all: simpl.
-    - unfold isPTyp.
-      change (S_Typ :: sc Γ) with (sc (Γ,,s (S_Typ, A))).
-      unfold sc. rewrite nth_error_map, H.
-      simpl. destruct s.
-      1: reflexivity.
-      destruct x.
-      + simpl in H. injection H.
-        discriminate.
-      + reflexivity.
-    - destruct s; reflexivity.
-    - injection eC; intros <- ->.
-      simpl.
-      destruct s.
-      + simpl in *; simpl.
-        f_equal.
-        
-
-        
-    inversion h3; subst.
-    2: reflexivity.
-    all: simpl.
-    - unfold isPTyp.
-      change (S_Typ :: sc Γ) with (sc (Γ,,s (S_Typ, A))).
-      unfold sc. rewrite nth_error_map, H1.
-      simpl. destruct s.
-      1: reflexivity.
-      destruct x.
-      + simpl in H1; injection H1.
-        discriminate.
-      + reflexivity.
-    - destruct s.
-      + simpl.
-  *)
-      
   Lemma tl_conv Γ u v :
+    swf Γ →
     u ≡ v →
     scoping (sc Γ) u S_PTyp →
     [ sc Γ | u ] ≡ [ sc Γ | v ].
   Proof.
-    intros h hP.
-    induction h in Γ, hP |- *.
-    - 
+    intros hΓ h hP.
+    induction h in Γ, hΓ, hP |- *.
+    - simpl. destruct s'.
+      1: apply scoping_st in hP; discriminate.
+      destruct s.
+      + eapply conv_trans.
+        1: eapply conv_beta.
+        admit.
+      + eapply conv_trans.
+        1: eapply conv_beta.
+        rewrite tl_subst with (Δ := S_PTyp :: sc Γ).
+        2: { apply σscoping_one. now inversion hP; subst. }
+        2: apply σscoping_comp_one.
+        2: { inversion hP; subst.
+             inversion H1; subst.
+             eapply scoping_subst.
+             2: eassumption.
+             now apply σscoping_one.
+        }
+        (*
+        assert
+            ([S_PTyp :: sc Γ | t] <[ u.. >> tl_tmP (sc Γ)] =
+             [S_PTyp :: sc Γ | t] <[ [ sc Γ | u].. ]) as ->.
+          {
+            change (S_PTyp :: sc Γ) with (sc (Γ,,s (S_PTyp, A))).
+            eapply tl_subst_ignore.
+            2: eassumption.
+            1, 2: econstructor; eassumption.
+            intros x hx.
+            destruct x.
+            1: reflexivity.
+            change ((u .. >> tl_tmP (sc Γ)) (S x)) with [sc Γ | var x ].
+            simpl. inversion hx; subst.
+            simpl in H0.
+            unfold isPTyp. rewrite H0.
+            reflexivity.
+          }
+         *)
   Admitted.
 
   (* main lemma for first translation *)
@@ -580,10 +519,18 @@ Section Translation.
             ([S_Typ :: sc Γ | B] <[ u.. >> tl_tmP (sc Γ)] =
              [S_Typ :: sc Γ | B] <[ [ sc Γ | u].. ]) as ->.
           {
-
-            change (u .. >> tl_tmP (sc Γ)) with
-              (λ x, [sc Γ | (u..) x ]).
-            admit. 
+            change (S_Typ :: sc Γ) with (sc (Γ,,s (S_Typ, A))).
+            eapply tl_subst_ignore.
+            2: eassumption.
+            1, 2: econstructor; eassumption.
+            intros x hx.
+            destruct x.
+            1: reflexivity.
+            change ((u .. >> tl_tmP (sc Γ)) (S x)) with [sc Γ | var x ].
+            simpl. inversion hx; subst.
+            simpl in H0.
+            unfold isPTyp. rewrite H0.
+            reflexivity.
           }
           assert ([S_Typ :: sc Γ | B] <[ [sc Γ | u]..] = [S_Typ :: sc Γ | B] <[ tt..]).
           {
@@ -622,8 +569,18 @@ Section Translation.
             ([S_PTyp :: sc Γ | B] <[ u.. >> tl_tmP (sc Γ)] =
              [S_PTyp :: sc Γ | B] <[ [ sc Γ | u].. ]) as ->.
           {
-            rasimpl.
-            admit.
+            change (S_PTyp :: sc Γ) with (sc (Γ,,s (S_PTyp, A))).
+            eapply tl_subst_ignore.
+            2: eassumption.
+            1, 2: econstructor; eassumption.
+            intros x hx.
+            destruct x.
+            1: reflexivity.
+            change ((u .. >> tl_tmP (sc Γ)) (S x)) with [sc Γ | var x ].
+            simpl. inversion hx; subst.
+            simpl in H0.
+            unfold isPTyp. rewrite H0.
+            reflexivity.
           }
           apply (ttype_app _ i j [sc Γ | A]).
           -- apply IHh1.
@@ -664,7 +621,7 @@ Section Translation.
       apply (ttype_conv _ i [sc Γ|A]).
       1: now apply IHh1.
       + apply tl_conv.
-        1: assumption.
+        all: try assumption.
         rewrite <-hP.
         now apply styping_scoping_stc_bw.
       + rewrite (styping_stc _ _ _ hΓ (stype_conv _ _ _ _ _ _ h1 H h2)) in hP.
@@ -675,8 +632,9 @@ Section Translation.
         1: assumption.
         change (S_PTyp) with (stc Γ (PTyp i)).
         now apply styping_scoping_stc.
-  Admitted.
+  Qed.
 
+  (*
   Lemma tl_unit_tt Γ u :
     scoping Γ u S_Typ →
     [Γ | u] = tt ∨ [Γ | u] = unit.
@@ -688,703 +646,105 @@ Section Translation.
     rewrite H.
     firstorder.
   Qed.
-
-  Lemma type_var_inv :
-  ∀ Γ x A,
-    Γ ⊢ var x : A →
-    ∃ s B,
-      nth_error Γ x = Some (s, B) ∧
-      (plus (S x)) ⋅ B ≡ A.
-  Proof.
-    intros Γ x A h.
-    dependent induction h.
-    all: try solve [discriminate].
-    - eexists _, _. split.
-      all: injection H0; intros ->.
-      1: eassumption.
-      constructor.
-    - destruct IHh1 as [s' [B' [h3 h4]]].
-      eexists _, _. split. 1: eassumption.
-      eapply conv_trans. all: eauto.
-  Qed.      
+   *)
   
-  (*
   Reserved Notation "⟦ Γ | t ⟧" (at level 0).
   Reserved Notation "⟦ Γ ⟧c" (at level 0).
+
+  Print ttyping.
+  
   
   Fixpoint Tl_tm (Γ : scope) (t : term) : term :=
     match t with
     | var x =>
-        unit
-        (* if (isPTyp Γ x) then sig [Γ|x] else tt *)
+        if (isPTyp Γ x) then (pi2 (var x)) else var x
 
     | Sort s i =>
 
         match s with
         | S_Typ => Typ i
-        | S_PTyp => lam_T (Typ i) (Pi_T i (S i) (var 0) (Typ i))
+        | S_PTyp =>
+            lam_T
+              [Γ | t] (*(Typ i)*)
+              (Pi_T i (S i) (var 0) (Typ i))
         end
 
-    | _ => unit
-    end.
-
-  (*
     | Pi s s' i j A B =>
-        match s' with
-        | S_Typ => unit
-        | S_PTyp =>
-            let A' :=
-              match s with
-              | S_Typ => unit
-              | S_PTyp => [Γ|A]
-              end in
-            Pi_T i j A' [Γ|B]
+
+        match s, s' with
+        | S_Typ, S_Typ =>
+            Pi_T i j ⟦Γ | A⟧ ⟦Γ | B⟧
+        | S_PTyp, S_Typ =>
+            Pi_T i j (Sigma [Γ | A] ⟦Γ | A⟧) ⟦Γ | B⟧
+        | S_PTyp, S_PTyp =>
+            lam_T
+              [Γ | t]
+              (Pi_T i j
+                 (Sigma [Γ | A] ⟦Γ | A⟧)
+                 (app_T ⟦Γ | B⟧ (app_T (var 1) (pi1 (var 0)))))
+        | S_Typ, S_PTyp =>
+            lam_T
+              [Γ | t]
+              (Pi_T i j
+                 ⟦Γ | A⟧
+                 (app_T ⟦Γ | B⟧ (app_T (var 1) (var 0))))
         end
-          
+
     | lam s s' A t =>
-        match s' with
-        | S_Typ => tt
-        | S_PTyp =>
-            let A' :=
-              match s with
-              | S_Typ => unit
-              | S_PTyp => [Γ|A]
-              end in
-            lam_T A' [Γ|t]
+        match s with
+        | S_Typ => lam_T ⟦Γ | A⟧ ⟦Γ | t⟧
+        | S_PTyp => lam_T (Sigma [Γ | A] ⟦Γ | A⟧) ⟦Γ | t⟧
         end
 
     | app s s' t u =>
-        match s' with
-        | S_Typ => tt
-        | S_PTyp =>
-            let u' :=
-              match s with
-              | S_Typ => tt
-              | S_PTyp => [Γ|u]
-              end in
-            app_T [Γ|t] u'
+        match s with
+        | S_Typ => app_T ⟦Γ | t⟧ ⟦Γ | u⟧
+        | S_PTyp => app_T ⟦Γ | t⟧ (sig [Γ | u] ⟦Γ | u⟧)
         end
 
-    | _ => unit (* inaccessible in styping *)                             
+    | _ => unit (* inaccessible in styping *)
     end
-*)
-  where "[ Γ | t ]" := (tl_tmP Γ t).
-      
-  Fixpoint tl_ctxP (Γ : sctx) : tctx :=
+  where "⟦ Γ | t ⟧" := (Tl_tm Γ t).
+
+  Fixpoint Tl_ctx (Γ : sctx) : tctx :=
     match Γ with
     | nil => ∙t
-    | cons (S_Typ, _) Γ => [Γ]c ,,t unit
-    | cons (S_PTyp, t) Γ => [Γ]c ,,t [sc Γ|t]
+    | cons (S_Typ, A) Γ => ⟦Γ⟧c ,,t ⟦sc Γ | A⟧
+    | cons (S_PTyp, A) Γ => ⟦Γ⟧c ,,t (Sigma [sc Γ | A] ⟦sc Γ | A⟧)
     end
-  where "[ Γ ]c" := (tl_ctxP Γ).
-   *)
-  
-End Translation.
+  where "⟦ Γ ⟧c" := (Tl_ctx Γ).
 
-(* Fixpoint tl_P *)
-  
-(*
-  Fixpoint inline (t : term) :=
-    match t with
-    | var n => var n
-    | Sort i => Sort i
-    | Pi A B => Pi ⟦ A ⟧ ⟦ B ⟧
-    | lam A t => lam ⟦ A ⟧ ⟦ t ⟧
-    | app u v => app ⟦ u ⟧ ⟦ v ⟧
-    | const c ξ => inst ⟦ ξ ⟧× (κ c)
-    | assm x => assm x
-    end
-
-  where "⟦ t ⟧" := (inline t)
-  and "⟦ k ⟧×" := (map_instance inline k).
-
-  Notation "⟦ l ⟧*" := (map inline l).
-
-  Definition inline_crule rule := {|
-    cr_env := ⟦ rule.(cr_env) ⟧* ;
-    cr_pat := ⟦ rule.(cr_pat) ⟧ ;
-    cr_sub := rule.(cr_sub) ;
-    cr_rep := ⟦ rule.(cr_rep) ⟧ ;
-    cr_typ := ⟦ rule.(cr_typ) ⟧
-  |}.
-
-  Notation "⟦ r ⟧r" := (inline_crule r).
-  Notation "⟦ R ⟧R" := (map inline_crule R).
-
-  Definition inline_idecl (d : idecl) :=
-    match d with
-    | Assm A => Assm ⟦ A ⟧
-    | Comp rl => Comp ⟦ rl ⟧r
+  Definition isPTyp_sc Γ t :=
+    match st Γ t with
+    | S_PTyp => true
+    | S_Typ => false
     end.
 
-  Notation "⟦ d ⟧d" := (inline_idecl d).
-  Notation "⟦ X ⟧e" := (map inline_idecl X).
+  Definition Tl_rhs Γ A t :=
+    if isPTyp_sc Γ t
+    then app_T ⟦Γ | A⟧ [Γ | t]
+    else ⟦Γ | A⟧.
 
-  Definition gclosed :=
-    ∀ c, closed (κ c) = true.
-
-  Context (hclosed : gclosed).
-
-  Lemma inline_ren ρ t :
-    ⟦ ρ ⋅ t ⟧ = ρ ⋅ ⟦ t ⟧.
+  Lemma isPTyp_sc_isPTyp Γ x :
+    isPTyp_sc Γ (var x) = isPTyp Γ x.
   Proof.
-    induction t in ρ |- * using term_rect.
-    all: try solve [ cbn ; f_equal ; eauto ].
-    cbn. rewrite ren_inst. rewrite closed_ren. 2: auto.
-    f_equal.
-    rewrite !map_map. apply map_ext_All.
-    eapply All_impl. 2: eassumption.
-    intros o h.
-    rewrite !option_map_option_map. apply option_map_ext_onSomeT.
-    eapply onSomeT_impl. 2: eassumption.
-    cbn. auto.
+    unfold isPTyp_sc.
+    unfold isPTyp. simpl.
+    rewrite nth_nth_error.
+    now destruct (nth_error Γ x).
   Qed.
-
-  Lemma up_term_inline σ n :
-    (up_term_term (σ >> inline)) n = (up_term_term σ >> inline) n.
+  
+  Lemma Tl_typ Γ t A :
+    swf Γ →
+    Γ ⊢ t : A →
+    ⟦ Γ ⟧c ⊨ ⟦sc Γ | t⟧ : Tl_rhs (sc Γ) A t.
   Proof.
-    rasimpl. destruct n.
-    - reflexivity.
-    - cbn. unfold core.funcomp. rewrite inline_ren. reflexivity.
-  Qed.
+    intros hΓ h.
+    induction h using styping_ind in hΓ |- *.
+    - simpl.
+      destruct (isPTyp (sc Γ) x) eqn: e.
+  Admitted.
 
-  Lemma inline_subst σ t :
-    ⟦ t <[ σ ] ⟧ = ⟦ t ⟧ <[ σ >> inline ].
-  Proof.
-    induction t in σ |- * using term_rect.
-    all: try solve [ cbn ; f_equal ; eauto ].
-    - cbn. f_equal. 1: eauto.
-      rewrite IHt2. eapply ext_term. intro.
-      rewrite up_term_inline. reflexivity.
-    - cbn. f_equal. 1: eauto.
-      rewrite IHt2. eapply ext_term. intro.
-      rewrite up_term_inline. reflexivity.
-    - cbn. rewrite subst_inst_closed. 2: auto.
-      f_equal.
-      rewrite !map_map. apply map_ext_All.
-      eapply All_impl. 2: eassumption.
-      intros ? h.
-      rewrite !option_map_option_map. apply option_map_ext_onSomeT.
-      eapply onSomeT_impl. 2: eassumption.
-      cbn. auto.
-  Qed.
-
-  Lemma inline_iget ξ x :
-    ⟦ iget ξ x ⟧ = iget ⟦ ξ ⟧× x.
-  Proof.
-    unfold iget. rewrite nth_error_map.
-    destruct nth_error as [[] |]. all: reflexivity.
-  Qed.
-
-  Lemma inline_ren_instance ρ ξ :
-    ⟦ ren_instance ρ ξ ⟧× = ren_instance ρ ⟦ ξ ⟧×.
-  Proof.
-    rewrite !map_map. apply map_ext. intro.
-    rewrite !option_map_option_map. apply option_map_ext. intro.
-    apply inline_ren.
-  Qed.
-
-  Lemma inline_inst ξ t :
-    ⟦ inst ξ t ⟧ = inst ⟦ ξ ⟧× ⟦ t ⟧.
-  Proof.
-    induction t in ξ |- * using term_rect.
-    all: try solve [ cbn ; f_equal ; eauto ].
-    - cbn. f_equal. 1: eauto.
-      rewrite IHt2. rewrite inline_ren_instance. reflexivity.
-    - cbn. f_equal. 1: eauto.
-      rewrite IHt2. rewrite inline_ren_instance. reflexivity.
-    - cbn. rewrite inst_inst. f_equal.
-      rewrite !map_map. apply map_ext_All.
-      eapply All_impl. 2: eassumption.
-      intros o ho. rewrite !option_map_option_map. apply option_map_ext_onSomeT.
-      eapply onSomeT_impl. 2: eassumption.
-      auto.
-    - cbn. apply inline_iget.
-  Qed.
-
-  Definition g_conv_unfold :=
-    ∀ c Ξ' A t,
-      Σ c = Some (Def Ξ' A t) →
-      [] ;; ⟦ Ξ' ⟧e ⊢ κ c ≡ ⟦ t ⟧.
-
-  Context (h_conv_unfold : g_conv_unfold).
-
-  Lemma conv_ren_inst Ξ ρ ξ ξ' :
-    Forall2 (option_rel (conversion Σ Ξ)) ξ ξ' →
-    Forall2 (option_rel (conversion Σ Ξ)) (ren_instance ρ ξ) (ren_instance ρ ξ').
-  Proof.
-    intros h.
-    apply Forall2_map_l, Forall2_map_r.
-    eapply Forall2_impl. 2: eassumption.
-    intros. apply option_rel_map_l, option_rel_map_r.
-    eapply option_rel_impl. 2: eassumption.
-    intros. eapply conv_ren. eassumption.
-  Qed.
-
-  Lemma ictx_get_assm_inline Ξ x A :
-    ictx_get Ξ x = Some (Assm A) →
-    ictx_get ⟦ Ξ ⟧e x = Some (Assm ⟦ A ⟧).
-  Proof.
-    intro h. rewrite ictx_get_map. rewrite h. reflexivity.
-  Qed.
-
-  Lemma ictx_get_comp_inline Ξ x rl :
-    ictx_get Ξ x = Some (Comp rl) →
-    ictx_get ⟦ Ξ ⟧e x = Some (Comp ⟦ rl ⟧r).
-  Proof.
-    intro h. rewrite ictx_get_map. rewrite h. reflexivity.
-  Qed.
-
-  Lemma scoped_instance_inline_ih k ξ :
-    All (onSomeT (λ t, ∀ k, scoped k t = true → scoped k ⟦ t ⟧ = true)) ξ →
-    scoped_instance k ξ = true →
-    scoped_instance k ⟦ ξ ⟧× = true.
-  Proof.
-    intros ih h.
-    apply forallb_All in h. move h at top.
-    eapply All_prod in h. 2: eassumption.
-    apply All_forallb. apply All_map. eapply All_impl. 2: eassumption.
-    cbn. intros o [h1 h2].
-    apply onSomeb_onSome, onSomeT_onSome. apply onSomeT_map.
-    apply onSomeb_onSome, onSome_onSomeT in h2.
-    eapply onSomeT_prod in h1. 2: eassumption.
-    eapply onSomeT_impl. 2: eassumption.
-    cbn. intros t []. eauto.
-  Qed.
-
-  Lemma scoped_inline k t :
-    scoped k t = true →
-    scoped k ⟦ t ⟧ = true.
-  Proof.
-    intros h.
-    induction t using term_rect in k, h |- *.
-    all: try solve [ cbn ; eauto ].
-    all: try solve [
-      cbn in * ; rewrite Bool.andb_true_iff in * ;
-      intuition eauto
-    ].
-    cbn in h |- *. eapply scoped_inst_closed.
-    - eapply scoped_instance_inline_ih. all: assumption.
-    - apply hclosed.
-  Qed.
-
-  Lemma scoped_instance_inline k ξ :
-    scoped_instance k ξ = true →
-    scoped_instance k ⟦ ξ ⟧× = true.
-  Proof.
-    intros h.
-    eapply scoped_instance_inline_ih. 2: assumption.
-    eapply forall_All. intros o ho.
-    destruct o. 2: constructor.
-    cbn. intros. eapply scoped_inline. assumption.
-  Qed.
-
-  Lemma iscope_instance_inline_ih Ξ ξ :
-    Forall (OnSome (λ t : term, iscope ⟦ Ξ ⟧e ⟦ t ⟧)) ξ →
-    iscope_instance ⟦ Ξ ⟧e ⟦ ξ ⟧×.
-  Proof.
-    intros ih.
-    apply Forall_map. eapply Forall_impl. 2: eassumption.
-    setoid_rewrite OnSome_onSome.
-    intros ??.
-    apply onSome_map.
-    eapply onSome_impl. 2: eassumption.
-    auto.
-  Qed.
-
-  Lemma iscope_inline Ξ t :
-    iscope Ξ t →
-    iscope ⟦ Ξ ⟧e ⟦ t ⟧.
-  Proof.
-    intros h.
-    induction h using iscope_ind_alt.
-    all: try solve [ cbn ; constructor; eauto ].
-    - cbn. eapply iscope_inst.
-      eauto using iscope_instance_inline_ih.
-    - cbn. econstructor.
-      eauto using ictx_get_assm_inline.
-  Qed.
-
-  Lemma inline_ctx_inst ξ Γ :
-    ⟦ ctx_inst ξ Γ ⟧* = ctx_inst ⟦ ξ ⟧× ⟦ Γ ⟧*.
-  Proof.
-    induction Γ as [| A Γ ih] in ξ |- *.
-    - reflexivity.
-    - cbn. rewrite ih. rewrite inline_inst.
-      rewrite inline_ren_instance. rewrite length_map. reflexivity.
-  Qed.
-
-  Lemma inst_equations_inline_ih Ξ Ξ' ξ :
-    inst_equations_ (λ u v, [] ;; ⟦ Ξ ⟧e ⊢ ⟦ u ⟧ ≡ ⟦ v ⟧) ξ Ξ' →
-    inst_equations [] ⟦ Ξ ⟧e ⟦ ξ ⟧× ⟦ Ξ' ⟧e.
-  Proof.
-    intros ih.
-    intros x rl hx.
-    rewrite ictx_get_map in hx.
-    destruct (ictx_get _ _) as [[| rl']|] eqn:hx'. 1,3: discriminate.
-    cbn in hx. inversion hx. subst. clear hx.
-    specialize (ih _ _ hx') as (hx & hl & hr & ih).
-    cbn. rewrite nth_error_map, hx. cbn.
-    rewrite !length_map.
-    rewrite !inline_inst in ih. rewrite !inline_ren_instance in ih.
-    intuition eauto using scoped_inline.
-  Qed.
-
-  Lemma cr_pat_inline rl :
-    ⟦ rl.(cr_pat) ⟧ = ⟦ rl ⟧r.(cr_pat).
-  Proof.
-    reflexivity.
-  Qed.
-
-  Lemma cr_rep_inline rl :
-    ⟦ rl.(cr_rep) ⟧ = ⟦ rl ⟧r.(cr_rep).
-  Proof.
-    reflexivity.
-  Qed.
-
-  Lemma conv_inline Ξ u v :
-    Σ ;; Ξ ⊢ u ≡ v →
-    [] ;; ⟦ Ξ ⟧e ⊢ ⟦ u ⟧ ≡ ⟦ v ⟧.
-  Proof.
-    intros h.
-    induction h using conversion_ind.
-    all: try solve [ cbn ; ttconv ].
-    - cbn. rewrite inline_subst. eapply meta_conv_trans_r. 1: econstructor.
-      apply ext_term. intros []. all: reflexivity.
-    - cbn. rewrite inline_inst. eapply conv_inst_closed.
-      + eapply inst_equations_inline_ih. eassumption.
-      + eapply h_conv_unfold. eassumption.
-    - rewrite !inline_subst. subst lhs rhs.
-      rewrite cr_pat_inline, cr_rep_inline.
-      eapply conv_red.
-      + apply ictx_get_comp_inline. eassumption.
-      + cbn. eapply scoped_inline. rewrite length_map. assumption.
-      + cbn. eapply scoped_inline. rewrite length_map. assumption.
-    - cbn. eapply conv_insts.
-      apply Forall2_map_l, Forall2_map_r.
-      eapply Forall2_impl. 2: eassumption.
-      intros. apply option_rel_map_l, option_rel_map_r.
-      eapply option_rel_impl. 2: eassumption.
-      cbn. auto.
-    - econstructor. assumption.
-    - eapply conv_trans. all: eassumption.
-  Qed.
-
-  Definition g_type :=
-    ∀ c Ξ' A t,
-      Σ c = Some (Def Ξ' A t) →
-      [] ;; ⟦ Ξ' ⟧e | ∙ ⊢ κ c : ⟦ A ⟧.
-
-  Context (h_type : g_type).
-
-  Lemma inst_typing_inline Ξ Γ ξ Ξ' :
-    iwf Σ Ξ' ->
-    inst_typing_ (conversion Σ Ξ) (λ t A, [] ;; ⟦ Ξ ⟧e | ⟦ Γ ⟧* ⊢ ⟦ t ⟧ : ⟦ A ⟧) ξ Ξ' →
-    inst_typing [] ⟦ Ξ ⟧e ⟦ Γ ⟧* ⟦ ξ ⟧× ⟦ Ξ' ⟧e.
-  Proof.
-    intro wf.
-    induction 1; cbn; depelim wf; try constructor; eauto.
-    - rewrite map_app; constructor; auto.
-      + apply scoped_inline. cbn.
-        now rewrite length_map.
-      + eapply iscope_inline. eassumption.
-      + apply scoped_inline. cbn.
-        now rewrite length_map.
-      + eapply iscope_inline. eassumption.
-      + cbn. rewrite !length_map.
-        rewrite <- !inline_ren_instance.
-        rewrite <- !inline_inst.
-        now apply conv_inline.
-    - rewrite map_app; constructor; auto.
-      + eapply iscope_inline. eassumption.
-      + apply scoped_inline. assumption.
-      + rewrite <- inline_inst. assumption.
-  Qed.
-
-  Lemma typing_inline Ξ Γ t A :
-    gwf Σ →
-    Σ ;; Ξ | Γ ⊢ t : A →
-    [] ;; ⟦ Ξ ⟧e | ⟦ Γ ⟧* ⊢ ⟦ t ⟧ : ⟦ A ⟧.
-  Proof.
-    intros hΣ h.
-    induction h using typing_ind.
-    all: try solve [ intros ; cbn ; tttype ].
-    - cbn. rewrite inline_ren. econstructor.
-      rewrite nth_error_map. rewrite H. reflexivity.
-    - cbn in *. eapply meta_conv.
-      + tttype.
-      + rewrite inline_subst. apply ext_term. intros []. all: reflexivity.
-    - apply valid_def in H as Hc; auto. destruct Hc as (wf & Hc).
-      cbn. rewrite inline_inst. eapply typing_inst_closed.
-      + eapply inst_typing_inline; eauto.
-      + eapply h_type. all: eassumption.
-    - cbn. econstructor.
-      + apply ictx_get_assm_inline. assumption.
-      + apply scoped_inline. assumption.
-    - econstructor. 1,3: eassumption.
-      apply conv_inline. assumption.
-  Qed.
-
-End Inline.
-
-Notation "⟦ t ⟧⟨ k ⟩" := (inline k t) (at level 0).
-Notation "⟦ l ⟧*⟨ k ⟩" := (map (inline k) l).
-Notation "⟦ t ⟧×⟨ k ⟩" := (map_instance (inline k) t).
-Notation "⟦ X ⟧e⟨ k ⟩" := (map (inline_idecl k) X).
-Notation "⟦ r ⟧r⟨ k ⟩" := (inline_crule k r).
-Notation "⟦ R ⟧R⟨ k ⟩" := (map (inline_crule k) R).
-
-Reserved Notation "⟦ s ⟧κ" (at level 0).
-
-(* TODO Probably can just use [list (greg * term)] *)
-
-Definition gnil (c : gref) :=
-  dummy.
-
-Definition gcons r t κ (c : gref) : term :=
-  if (c =? r)%string then t else κ c.
-
-Fixpoint inline_gctx_ufd Σ :=
-  match Σ with
-  | (c, d) :: Σ =>
-    let κ := ⟦ Σ ⟧κ in
-    match d with
-    | Def Ξ A t => gcons c ⟦ t ⟧⟨ κ ⟩ κ
-    end
-  | [] => gnil
-  end
-where "⟦ s ⟧κ" := (inline_gctx_ufd s).
-
-Lemma gcons_eq c c' t κ :
-  (c' =? c)%string = true →
-  gcons c t κ c' = t.
-Proof.
-  intro h.
-  unfold gcons. rewrite h. reflexivity.
-Qed.
-
-Lemma gcons_neq c c' t κ :
-  (c' =? c)%string = false →
-  gcons c t κ c' = κ c'.
-Proof.
-  intro h.
-  unfold gcons. rewrite h. reflexivity.
-Qed.
-
-Definition eq_gscope (Σ : gctx) (κ κ' : ginst) :=
-  ∀ c Ξ' A t,
-    Σ c = Some (Def Ξ' A t) →
-    κ c = κ' c.
-
-Lemma inline_ext Σ t κ κ' :
-  gscope Σ t →
-  eq_gscope Σ κ κ' →
-  ⟦ t ⟧⟨ κ ⟩ = ⟦ t ⟧⟨ κ' ⟩.
-Proof.
-  intros ht he.
-  induction ht in κ, κ', he |- * using gscope_ind.
-  all: try solve [ cbn ; eauto ].
-  all: try solve [ cbn ; f_equal ; eauto ].
-  cbn.
-  assert (e : ⟦ ξ ⟧×⟨ κ ⟩ = ⟦ ξ ⟧×⟨ κ' ⟩).
-  { apply map_ext_Forall. eapply Forall_impl. 2: eassumption.
-    intros o ho.
-    rewrite OnSome_onSome in ho. apply onSome_onSomeT in ho.
-    apply option_map_ext_onSomeT. eapply onSomeT_impl. 2: eassumption.
-    cbn. auto.
-  }
-  rewrite <- e. f_equal.
-  eapply he. eassumption.
-Qed.
-
-Lemma inline_instance_ext Σ (ξ : instance) κ κ' :
-  gscope_instance Σ ξ →
-  eq_gscope Σ κ κ' →
-  ⟦ ξ ⟧×⟨ κ ⟩ = ⟦ ξ ⟧×⟨ κ' ⟩.
-Proof.
-  intros hξ he.
-  eapply map_ext_Forall. eapply Forall_impl. 2: eassumption.
-  intros o ho. rewrite OnSome_onSome in ho. apply onSome_onSomeT in ho.
-  eapply option_map_ext_onSomeT. eapply onSomeT_impl. 2: eassumption.
-  intros. eapply inline_ext. all: eassumption.
-Qed.
-
-Lemma inline_list_ext Σ l κ κ' :
-  Forall (gscope Σ) l →
-  eq_gscope Σ κ κ' →
-  ⟦ l ⟧*⟨ κ ⟩ = ⟦ l ⟧*⟨ κ' ⟩.
-Proof.
-  intros hl he.
-  eapply map_ext_Forall. eapply Forall_impl. 2: eassumption.
-  intros. eapply inline_ext. all: eassumption.
-Qed.
-
-Lemma inline_crule_ext Σ rl κ κ' :
-  gscope_crule Σ rl →
-  eq_gscope Σ κ κ' →
-  ⟦ rl ⟧r⟨ κ ⟩ = ⟦ rl ⟧r⟨ κ' ⟩.
-Proof.
-  intros [? [? []]] he.
-  destruct rl as [Θ l r θ A].
-  unfold inline_crule. cbn in *. f_equal.
-  - eapply inline_list_ext. all: eassumption.
-  - eapply inline_ext. all: eassumption.
-  - eapply inline_ext. all: eassumption.
-  - eapply inline_ext. all: eassumption.
-Qed.
-
-Lemma inline_crules_ext Σ R κ κ' :
-  Forall (gscope_crule Σ) R →
-  eq_gscope Σ κ κ' →
-  ⟦ R ⟧R⟨ κ ⟩ = ⟦ R ⟧R⟨ κ' ⟩.
-Proof.
-  intros hR he.
-  eapply map_ext_Forall. eapply Forall_impl. 2: eassumption.
-  intros. eapply inline_crule_ext. all: eassumption.
-Qed.
-
-Lemma inline_ictx_ext Σ Ξ κ κ' :
-  iwf Σ Ξ →
-  eq_gscope Σ κ κ' →
-  ⟦ Ξ ⟧e⟨ κ ⟩ = ⟦ Ξ ⟧e⟨ κ' ⟩.
-Proof.
-  intros hΞ he.
-  eapply map_ext_Forall.
-  induction hΞ as [| B Ξ i hΞ ih hB | rl Ξ hΞ ih hs ht ].
-  - constructor.
-  - constructor. 2: assumption.
-    cbn. f_equal. eapply inline_ext. 2: eassumption.
-    eapply typing_gscope. eassumption.
-  - constructor. 2: assumption.
-    cbn. f_equal. eapply inline_crule_ext. all: eassumption.
-Qed.
-
-Lemma inline_ctx_ext Σ Ξ Γ κ κ' :
-  wf Σ Ξ Γ →
-  eq_gscope Σ κ κ' →
-  ⟦ Γ ⟧*⟨ κ ⟩ = ⟦ Γ ⟧*⟨ κ' ⟩.
-Proof.
-  intros hΓ he.
-  eapply inline_list_ext. 2: eassumption.
-  eapply wf_gscope. eassumption.
-Qed.
-
-Lemma eq_gscope_gcons (Σ : gctx) κ c u :
-  Σ c = None →
-  eq_gscope Σ κ (gcons c u κ).
-Proof.
-  intros h c' Ξ A t e.
-  destruct (c' =? c)%string eqn:ec.
-  1:{ rewrite String.eqb_eq in ec. congruence. }
-  rewrite gcons_neq. 2: assumption.
-  reflexivity.
-Qed.
-
-Lemma gwf_gclosed Σ :
-  gwf Σ →
-  gclosed ⟦ Σ ⟧κ.
-Proof.
-  intros h.
-  induction h as [ | c' ??????? ih ].
-  all: intros c.
-  - cbn. reflexivity.
-  - cbn. destruct (c =? c')%string eqn:ec.
-    + rewrite gcons_eq. 2: assumption.
-      eapply scoped_inline. 1: assumption.
-      eapply typing_closed. eassumption.
-    + rewrite gcons_neq. 2: assumption.
-      eauto.
-Qed.
-
-Lemma gwf_conv_unfold Σ :
-  gwf Σ →
-  g_conv_unfold Σ ⟦ Σ ⟧κ.
-Proof.
-  intros h c Ξ' A t ec.
-  apply meta_conv_refl.
-  induction h as [ | c' ??????? ih ].
-  - discriminate.
-  - cbn in *. destruct (c =? c')%string eqn:e.
-    + inversion ec. subst. clear ec.
-      rewrite gcons_eq. 2: assumption.
-      eapply inline_ext.
-      all: eauto using eq_gscope_gcons, typing_gscope.
-    + rewrite gcons_neq. 2: assumption.
-      eapply valid_def in ec as h'. 2: assumption.
-      destruct h' as (hΞ' & [j hB] & ht).
-      erewrite <- inline_ext.
-      2,3: eauto using eq_gscope_gcons, typing_gscope.
-      eauto.
-Qed.
-
-Lemma gwf_type Σ :
-  gwf Σ →
-  g_type Σ ⟦ Σ ⟧κ.
-Proof.
-  intros h.
-  induction h as [ | c' ??????? ih ].
-  all: intros c Ξ' B u ec.
-  - discriminate.
-  - cbn in *. destruct (c =? c')%string eqn:e.
-    + inversion ec. subst. clear ec.
-      rewrite gcons_eq. 2: assumption.
-      erewrite <- inline_ictx_ext. 2,3: eauto using eq_gscope_gcons.
-      erewrite <- inline_ext with (t := B).
-      2,3: eauto using eq_gscope_gcons, typing_gscope.
-      eapply typing_inline with (Γ := ∙).
-      * eapply gwf_gclosed. assumption.
-      * eapply gwf_conv_unfold. assumption.
-      * assumption.
-      * assumption.
-      * assumption.
-    + rewrite gcons_neq. 2: assumption.
-      eapply valid_def in ec as h'. 2: assumption.
-      destruct h' as (hΞ' & [j hB] & ht).
-      erewrite <- inline_ictx_ext. 2,3: eauto using eq_gscope_gcons.
-      erewrite <- inline_ext with (t := B).
-      2,3: eauto using eq_gscope_gcons, typing_gscope.
-      eauto.
-Qed.
-
-Theorem inlining Ξ Σ Γ t A :
-  gwf Σ →
-  let κ := ⟦ Σ ⟧κ in
-  Σ ;; Ξ | Γ ⊢ t : A →
-  [] ;; ⟦ Ξ ⟧e⟨ κ ⟩ | ⟦ Γ ⟧*⟨ κ ⟩ ⊢ ⟦ t ⟧⟨ κ ⟩ : ⟦ A ⟧⟨ κ ⟩.
-Proof.
-  intros hΣ κ h.
-  eapply typing_inline.
-  - eapply gwf_gclosed. assumption.
-  - eapply gwf_conv_unfold. assumption.
-  - eapply gwf_type. assumption.
-  - assumption.
-  - assumption.
-Qed.
-
-(** Conservativity *)
-
-Lemma inline_nil_id t κ :
-  gscope [] t →
-  ⟦ t ⟧⟨ κ ⟩ = t.
-Proof.
-  intros h. induction h using gscope_ind.
-  all: try solve [ cbn ; f_equal ; eauto ].
-  discriminate.
-Qed.
-
-Theorem conservativity Σ t A i :
-  gwf Σ →
-  [] ;; [] | ∙ ⊢ A : Sort i →
-  Σ ;; [] | ∙ ⊢ t : A →
-  let κ := ⟦ Σ ⟧κ in
-  [] ;; [] | ∙ ⊢ ⟦ t ⟧⟨ κ ⟩ : A.
-Proof.
-  intros hΣ hA ht κ.
-  eapply inlining in ht. 2: assumption.
-  cbn in ht.
-  eapply typing_gscope in hA as gA. eapply inline_nil_id in gA.
-  rewrite gA in ht. eassumption.
-Qed.
-
-
-*)
+  
+    
+End Translation.
